Clean up, prepare tests

Lynx/Term.lean
@@ -1,13 +1,5 @@
 namespace Lynx
 
-/-!
-Runtime Elixir values used by our first semantic fragment.
-
-Elixir lists are not a special host-language `List Term`. They are constructed
-from `nil` and cons cells. Consequently, this type can also represent improper
-lists such as `[1 | 2]`.
--/
-
 inductive Term where
   | integer : Int → Term
   | atom : String → Term
@@ -15,15 +7,53 @@ inductive Term where
   | cons : Term → Term → Term
 deriving Repr, DecidableEq
 
+namespace Term
+
+def «true» : Term :=
+  .atom "true"
+
+def «false» : Term :=
+  .atom "false"
+
+end Term
+
 inductive Exception where
   | error : Term → Exception
   | throw : Term → Exception
   | exit : Term → Exception
 deriving Repr, DecidableEq
 
-inductive Outcome where
-  | value : Term → Outcome
-  | raised : Exception → Outcome
+inductive Outcome (α : Type) where
+  | value : α → Outcome α
+  | raised : Exception → Outcome α
 deriving Repr, DecidableEq
+
+instance : Monad Outcome where
+  pure := .value
+  bind outcome next :=
+    match outcome with
+    | .value value => next value
+    | .raised exception => .raised exception
+
+instance : MonadExceptOf Exception Outcome where
+  throw := .raised
+  tryCatch outcome handler :=
+    match outcome with
+    | .value value => .value value
+    | .raised exception => handler exception
+
+@[simp] theorem Outcome.value_bind
+    (value : α) (next : α → Outcome β) :
+    (Outcome.value value >>= next) = next value :=
+  rfl
+
+@[simp] theorem Outcome.raised_bind
+    (exception : Exception) (next : α → Outcome β) :
+    (Outcome.raised exception >>= next) = .raised exception :=
+  rfl
+
+@[simp] theorem Outcome.throw_eq (exception : Exception) :
+    (throw exception : Outcome α) = .raised exception :=
+  rfl
 
 end Lynx
