Lynx.lean
@@ -1,4 +1,3 @@
 import Lynx.Term
 import Lynx.Contract
-import Lynx.Examples.LeanSum
-import Lynx.Examples.TermSum
+import Lynx.Modules.Erlang
