Main.lean
@@ -1,5 +1,0 @@
-import Lynx
-
-def main : IO Unit :=
-  IO.println s!"{repr (Lynx.Examples.TermSum.sumTerm
-    (Lynx.Examples.TermSum.encodeIntList [1, 2, 3]))}"
